Several improvements and fixes of Lia
- Improved reification for Micromega (support for #8764)

- Fixes #9268: Do not take universes into account in lia reification

  Improve #9291 by threading the evar_map during reification.
  Universes are unified.

- Remove (potentially cyclic) dependency over lra for Rle_abs

- Towards a complete simplex-based lia

  fixes  #9615

Lia is now exclusively using cutting plane proofs.
For this to always work, all the variables need to be positive.
Therefore, lia is pre-processing the goal  for each variable x
it introduces the constraints x = y - z , y>=0 , z >= 0
for some fresh variable y and z.

For scalability, nia is currently NOT performing this pre-processing.

- Lia is using the FSet library

  manual merge of commit #230899e87c51c12b2f21b6fedc414d099a1425e4
  to work around a "leaked" hint breaking compatibility of eauto

plugins/micromega/certificate.mli
@@ -15,6 +15,15 @@ module Mc = Micromega
     If set, use the Simplex method, otherwise use Fourier *)
 val use_simplex : bool ref
 
+type ('prf,'model) res =
+   | Prf of 'prf
+   | Model of 'model
+   | Unknown
+
+type zres = (Mc.zArithProof , (int * Mc.z  list)) res
+
+type qres = (Mc.q Mc.psatz , (int * Mc.q  list)) res
+
 (** [dump_file] is bound to the Coq option Dump Arith.
     If set to some [file], arithmetic goals are dumped in filexxx.v *)
 val dump_file : string option ref
@@ -27,16 +36,16 @@ val z_cert_of_pos : Sos_types.positivstellensatz -> Mc.z Mc.psatz
 
 (** [lia enum depth sys] generates an unsat proof for the linear constraints in [sys].
     If the Simplex option is set, any failure to find a proof should be considered as a bug. *)
-val lia : bool -> int -> (Mc.z Mc.pExpr * Mc.op1) list -> Mc.zArithProof option
+val lia : bool -> int -> (Mc.z Mc.pExpr * Mc.op1) list -> zres
 
 (** [nlia enum depth sys] generates an unsat proof for the non-linear constraints in [sys].
     The solver is incomplete -- the problem is undecidable *)
-val nlia : bool -> int -> (Mc.z Mc.pExpr * Mc.op1) list -> Mc.zArithProof option
+val nlia : bool -> int -> (Mc.z Mc.pExpr * Mc.op1) list -> zres
 
 (** [linear_prover_with_cert depth sys] generates an unsat proof for the linear constraints in [sys].
     Over the rationals, the solver is complete. *)
-val linear_prover_with_cert : int -> (Mc.q Mc.pExpr * Mc.op1) list -> Mc.q Micromega.psatz option
+val linear_prover_with_cert : int -> (Mc.q Mc.pExpr * Mc.op1) list -> qres
 
 (** [nlinear depth sys] generates an unsat proof for the non-linear constraints in [sys].
     The solver is incompete -- the problem is decidable. *)
-val nlinear_prover : int -> (Mc.q Mc.pExpr * Mc.op1) list -> Mc.q Mc.psatz option
+val nlinear_prover : int -> (Mc.q Mc.pExpr * Mc.op1) list -> qres
