plugins/micromega/micromega.mli
@@ -1,9 +1,22 @@
 
+type __ = Obj.t
+
+type unit0 =
+| Tt
+
 val negb : bool -> bool
 
 type nat =
 | O
 | S of nat
+
+type ('a, 'b) sum =
+| Inl of 'a
+| Inr of 'b
+
+val fst : ('a1 * 'a2) -> 'a1
+
+val snd : ('a1 * 'a2) -> 'a2
 
 val app : 'a1 list -> 'a1 list -> 'a1 list
 
@@ -15,6 +28,12 @@ type comparison =
 val compOpp : comparison -> comparison
 
 val add : nat -> nat -> nat
+
+val nth : nat -> 'a1 list -> 'a1 -> 'a1
+
+val map : ('a1 -> 'a2) -> 'a1 list -> 'a2 list
+
+val fold_right : ('a2 -> 'a1 -> 'a1) -> 'a1 -> 'a2 list -> 'a1
 
 type positive =
 | XI of positive
@@ -87,12 +106,6 @@ module N :
 
 val pow_pos : ('a1 -> 'a1 -> 'a1) -> 'a1 -> positive -> 'a1
 
-val nth : nat -> 'a1 list -> 'a1 -> 'a1
-
-val map : ('a1 -> 'a2) -> 'a1 list -> 'a2 list
-
-val fold_right : ('a2 -> 'a1 -> 'a1) -> 'a1 -> 'a2 list -> 'a1
-
 module Z :
  sig
   val double : z -> z
@@ -124,6 +137,8 @@ module Z :
   val abs : z -> z
 
   val to_N : z -> n
+
+  val of_nat : nat -> z
 
   val pos_div_eucl : positive -> z -> z * z
 
@@ -163,27 +178,47 @@ val paddC : ('a1 -> 'a1 -> 'a1) -> 'a1 pol -> 'a1 -> 'a1 pol
 
 val psubC : ('a1 -> 'a1 -> 'a1) -> 'a1 pol -> 'a1 -> 'a1 pol
 
-val paddI : ('a1 -> 'a1 -> 'a1) -> ('a1 pol -> 'a1 pol -> 'a1 pol) -> 'a1 pol -> positive -> 'a1 pol -> 'a1 pol
+val paddI :
+  ('a1 -> 'a1 -> 'a1) -> ('a1 pol -> 'a1 pol -> 'a1 pol) -> 'a1 pol -> positive -> 'a1
+  pol -> 'a1 pol
 
-val psubI : ('a1 -> 'a1 -> 'a1) -> ('a1 -> 'a1) -> ('a1 pol -> 'a1 pol -> 'a1 pol) -> 'a1 pol -> positive -> 'a1 pol -> 'a1 pol
+val psubI :
+  ('a1 -> 'a1 -> 'a1) -> ('a1 -> 'a1) -> ('a1 pol -> 'a1 pol -> 'a1 pol) -> 'a1 pol ->
+  positive -> 'a1 pol -> 'a1 pol
 
-val paddX : 'a1 -> ('a1 -> 'a1 -> bool) -> ('a1 pol -> 'a1 pol -> 'a1 pol) -> 'a1 pol -> positive -> 'a1 pol -> 'a1 pol
+val paddX :
+  'a1 -> ('a1 -> 'a1 -> bool) -> ('a1 pol -> 'a1 pol -> 'a1 pol) -> 'a1 pol ->
+  positive -> 'a1 pol -> 'a1 pol
 
-val psubX : 'a1 -> ('a1 -> 'a1) -> ('a1 -> 'a1 -> bool) -> ('a1 pol -> 'a1 pol -> 'a1 pol) -> 'a1 pol -> positive -> 'a1 pol -> 'a1 pol
+val psubX :
+  'a1 -> ('a1 -> 'a1) -> ('a1 -> 'a1 -> bool) -> ('a1 pol -> 'a1 pol -> 'a1 pol) ->
+  'a1 pol -> positive -> 'a1 pol -> 'a1 pol
 
-val padd : 'a1 -> ('a1 -> 'a1 -> 'a1) -> ('a1 -> 'a1 -> bool) -> 'a1 pol -> 'a1 pol -> 'a1 pol
+val padd :
+  'a1 -> ('a1 -> 'a1 -> 'a1) -> ('a1 -> 'a1 -> bool) -> 'a1 pol -> 'a1 pol -> 'a1 pol
 
-val psub : 'a1 -> ('a1 -> 'a1 -> 'a1) -> ('a1 -> 'a1 -> 'a1) -> ('a1 -> 'a1) -> ('a1 -> 'a1 -> bool) -> 'a1 pol -> 'a1 pol -> 'a1 pol
+val psub :
+  'a1 -> ('a1 -> 'a1 -> 'a1) -> ('a1 -> 'a1 -> 'a1) -> ('a1 -> 'a1) -> ('a1 -> 'a1 ->
+  bool) -> 'a1 pol -> 'a1 pol -> 'a1 pol
 
-val pmulC_aux : 'a1 -> ('a1 -> 'a1 -> 'a1) -> ('a1 -> 'a1 -> bool) -> 'a1 pol -> 'a1 -> 'a1 pol
+val pmulC_aux :
+  'a1 -> ('a1 -> 'a1 -> 'a1) -> ('a1 -> 'a1 -> bool) -> 'a1 pol -> 'a1 -> 'a1 pol
 
-val pmulC : 'a1 -> 'a1 -> ('a1 -> 'a1 -> 'a1) -> ('a1 -> 'a1 -> bool) -> 'a1 pol -> 'a1 -> 'a1 pol
+val pmulC :
+  'a1 -> 'a1 -> ('a1 -> 'a1 -> 'a1) -> ('a1 -> 'a1 -> bool) -> 'a1 pol -> 'a1 -> 'a1
+  pol
 
-val pmulI : 'a1 -> 'a1 -> ('a1 -> 'a1 -> 'a1) -> ('a1 -> 'a1 -> bool) -> ('a1 pol -> 'a1 pol -> 'a1 pol) -> 'a1 pol -> positive -> 'a1 pol -> 'a1 pol
+val pmulI :
+  'a1 -> 'a1 -> ('a1 -> 'a1 -> 'a1) -> ('a1 -> 'a1 -> bool) -> ('a1 pol -> 'a1 pol ->
+  'a1 pol) -> 'a1 pol -> positive -> 'a1 pol -> 'a1 pol
 
-val pmul : 'a1 -> 'a1 -> ('a1 -> 'a1 -> 'a1) -> ('a1 -> 'a1 -> 'a1) -> ('a1 -> 'a1 -> bool) -> 'a1 pol -> 'a1 pol -> 'a1 pol
+val pmul :
+  'a1 -> 'a1 -> ('a1 -> 'a1 -> 'a1) -> ('a1 -> 'a1 -> 'a1) -> ('a1 -> 'a1 -> bool) ->
+  'a1 pol -> 'a1 pol -> 'a1 pol
 
-val psquare : 'a1 -> 'a1 -> ('a1 -> 'a1 -> 'a1) -> ('a1 -> 'a1 -> 'a1) -> ('a1 -> 'a1 -> bool) -> 'a1 pol -> 'a1 pol
+val psquare :
+  'a1 -> 'a1 -> ('a1 -> 'a1 -> 'a1) -> ('a1 -> 'a1 -> 'a1) -> ('a1 -> 'a1 -> bool) ->
+  'a1 pol -> 'a1 pol
 
 type 'c pExpr =
 | PEc of 'c
@@ -197,49 +232,104 @@ type 'c pExpr =
 val mk_X : 'a1 -> 'a1 -> positive -> 'a1 pol
 
 val ppow_pos :
-  'a1 -> 'a1 -> ('a1 -> 'a1 -> 'a1) -> ('a1 -> 'a1 -> 'a1) -> ('a1 -> 'a1 -> bool) -> ('a1 pol -> 'a1 pol) -> 'a1 pol -> 'a1 pol -> positive -> 'a1 pol
+  'a1 -> 'a1 -> ('a1 -> 'a1 -> 'a1) -> ('a1 -> 'a1 -> 'a1) -> ('a1 -> 'a1 -> bool) ->
+  ('a1 pol -> 'a1 pol) -> 'a1 pol -> 'a1 pol -> positive -> 'a1 pol
 
-val ppow_N : 'a1 -> 'a1 -> ('a1 -> 'a1 -> 'a1) -> ('a1 -> 'a1 -> 'a1) -> ('a1 -> 'a1 -> bool) -> ('a1 pol -> 'a1 pol) -> 'a1 pol -> n -> 'a1 pol
+val ppow_N :
+  'a1 -> 'a1 -> ('a1 -> 'a1 -> 'a1) -> ('a1 -> 'a1 -> 'a1) -> ('a1 -> 'a1 -> bool) ->
+  ('a1 pol -> 'a1 pol) -> 'a1 pol -> n -> 'a1 pol
 
 val norm_aux :
-  'a1 -> 'a1 -> ('a1 -> 'a1 -> 'a1) -> ('a1 -> 'a1 -> 'a1) -> ('a1 -> 'a1 -> 'a1) -> ('a1 -> 'a1) -> ('a1 -> 'a1 -> bool) -> 'a1 pExpr -> 'a1 pol
+  'a1 -> 'a1 -> ('a1 -> 'a1 -> 'a1) -> ('a1 -> 'a1 -> 'a1) -> ('a1 -> 'a1 -> 'a1) ->
+  ('a1 -> 'a1) -> ('a1 -> 'a1 -> bool) -> 'a1 pExpr -> 'a1 pol
 
-type 'a bFormula =
+type ('tA, 'tX, 'aA, 'aF) gFormula =
 | TT
 | FF
-| X
-| A of 'a
-| Cj of 'a bFormula * 'a bFormula
-| D of 'a bFormula * 'a bFormula
-| N of 'a bFormula
-| I of 'a bFormula * 'a bFormula
+| X of 'tX
+| A of 'tA * 'aA
+| Cj of ('tA, 'tX, 'aA, 'aF) gFormula * ('tA, 'tX, 'aA, 'aF) gFormula
+| D of ('tA, 'tX, 'aA, 'aF) gFormula * ('tA, 'tX, 'aA, 'aF) gFormula
+| N of ('tA, 'tX, 'aA, 'aF) gFormula
+| I of ('tA, 'tX, 'aA, 'aF) gFormula * 'aF option * ('tA, 'tX, 'aA, 'aF) gFormula
 
-val map_bformula : ('a1 -> 'a2) -> 'a1 bFormula -> 'a2 bFormula
+val mapX :
+  ('a2 -> 'a2) -> ('a1, 'a2, 'a3, 'a4) gFormula -> ('a1, 'a2, 'a3, 'a4) gFormula
 
-type 'x clause = 'x list
+val foldA : ('a5 -> 'a3 -> 'a5) -> ('a1, 'a2, 'a3, 'a4) gFormula -> 'a5 -> 'a5
 
-type 'x cnf = 'x clause list
+val cons_id : 'a1 option -> 'a1 list -> 'a1 list
 
-val tt : 'a1 cnf
+val ids_of_formula : ('a1, 'a2, 'a3, 'a4) gFormula -> 'a4 list
 
-val ff : 'a1 cnf
+val collect_annot : ('a1, 'a2, 'a3, 'a4) gFormula -> 'a3 list
 
-val add_term : ('a1 -> bool) -> ('a1 -> 'a1 -> 'a1 option) -> 'a1 -> 'a1 clause -> 'a1 clause option
+type 'a bFormula = ('a, __, unit0, unit0) gFormula
 
-val or_clause : ('a1 -> bool) -> ('a1 -> 'a1 -> 'a1 option) -> 'a1 clause -> 'a1 clause -> 'a1 clause option
+val map_bformula :
+  ('a1 -> 'a2) -> ('a1, 'a3, 'a4, 'a5) gFormula -> ('a2, 'a3, 'a4, 'a5) gFormula
 
-val or_clause_cnf : ('a1 -> bool) -> ('a1 -> 'a1 -> 'a1 option) -> 'a1 clause -> 'a1 cnf -> 'a1 cnf
+type ('x, 'annot) clause = ('x * 'annot) list
 
-val or_cnf : ('a1 -> bool) -> ('a1 -> 'a1 -> 'a1 option) -> 'a1 cnf -> 'a1 cnf -> 'a1 cnf
+type ('x, 'annot) cnf = ('x, 'annot) clause list
 
-val and_cnf : 'a1 cnf -> 'a1 cnf -> 'a1 cnf
+val cnf_tt : ('a1, 'a2) cnf
 
-val xcnf : ('a2 -> bool) -> ('a2 -> 'a2 -> 'a2 option) -> ('a1 -> 'a2 cnf) -> ('a1 -> 'a2 cnf) -> bool -> 'a1 bFormula -> 'a2 cnf
+val cnf_ff : ('a1, 'a2) cnf
 
-val cnf_checker : ('a1 list -> 'a2 -> bool) -> 'a1 cnf -> 'a2 list -> bool
+val add_term :
+  ('a1 -> bool) -> ('a1 -> 'a1 -> 'a1 option) -> ('a1 * 'a2) -> ('a1, 'a2) clause ->
+  ('a1, 'a2) clause option
+
+val or_clause :
+  ('a1 -> bool) -> ('a1 -> 'a1 -> 'a1 option) -> ('a1, 'a2) clause -> ('a1, 'a2)
+  clause -> ('a1, 'a2) clause option
+
+val or_clause_cnf :
+  ('a1 -> bool) -> ('a1 -> 'a1 -> 'a1 option) -> ('a1, 'a2) clause -> ('a1, 'a2) cnf
+  -> ('a1, 'a2) cnf
+
+val or_cnf :
+  ('a1 -> bool) -> ('a1 -> 'a1 -> 'a1 option) -> ('a1, 'a2) cnf -> ('a1, 'a2) cnf ->
+  ('a1, 'a2) cnf
+
+val and_cnf : ('a1, 'a2) cnf -> ('a1, 'a2) cnf -> ('a1, 'a2) cnf
+
+type ('term, 'annot, 'tX, 'aF) tFormula = ('term, 'tX, 'annot, 'aF) gFormula
+
+val xcnf :
+  ('a2 -> bool) -> ('a2 -> 'a2 -> 'a2 option) -> ('a1 -> 'a3 -> ('a2, 'a3) cnf) ->
+  ('a1 -> 'a3 -> ('a2, 'a3) cnf) -> bool -> ('a1, 'a3, 'a4, 'a5) tFormula -> ('a2,
+  'a3) cnf
+
+val radd_term :
+  ('a1 -> bool) -> ('a1 -> 'a1 -> 'a1 option) -> ('a1 * 'a2) -> ('a1, 'a2) clause ->
+  (('a1, 'a2) clause, 'a2 list) sum
+
+val ror_clause :
+  ('a1 -> bool) -> ('a1 -> 'a1 -> 'a1 option) -> ('a1 * 'a2) list -> ('a1, 'a2) clause
+  -> (('a1, 'a2) clause, 'a2 list) sum
+
+val ror_clause_cnf :
+  ('a1 -> bool) -> ('a1 -> 'a1 -> 'a1 option) -> ('a1 * 'a2) list -> ('a1, 'a2) clause
+  list -> ('a1, 'a2) clause list * 'a2 list
+
+val ror_cnf :
+  ('a1 -> bool) -> ('a1 -> 'a1 -> 'a1 option) -> ('a1 * 'a2) list list -> ('a1, 'a2)
+  clause list -> ('a1, 'a2) cnf * 'a2 list
+
+val rxcnf :
+  ('a2 -> bool) -> ('a2 -> 'a2 -> 'a2 option) -> ('a1 -> 'a3 -> ('a2, 'a3) cnf) ->
+  ('a1 -> 'a3 -> ('a2, 'a3) cnf) -> bool -> ('a1, 'a3, 'a4, 'a5) tFormula -> ('a2,
+  'a3) cnf * 'a3 list
+
+val cnf_checker :
+  (('a1 * 'a2) list -> 'a3 -> bool) -> ('a1, 'a2) cnf -> 'a3 list -> bool
 
 val tauto_checker :
-  ('a2 -> bool) -> ('a2 -> 'a2 -> 'a2 option) -> ('a1 -> 'a2 cnf) -> ('a1 -> 'a2 cnf) -> ('a2 list -> 'a3 -> bool) -> 'a1 bFormula -> 'a3 list -> bool
+  ('a2 -> bool) -> ('a2 -> 'a2 -> 'a2 option) -> ('a1 -> 'a3 -> ('a2, 'a3) cnf) ->
+  ('a1 -> 'a3 -> ('a2, 'a3) cnf) -> (('a2 * 'a3) list -> 'a4 -> bool) -> ('a1, __,
+  'a3, unit0) gFormula -> 'a4 list -> bool
 
 val cneqb : ('a1 -> 'a1 -> bool) -> 'a1 -> 'a1 -> bool
 
@@ -273,21 +363,27 @@ val map_option : ('a1 -> 'a2 option) -> 'a1 option -> 'a2 option
 val map_option2 : ('a1 -> 'a2 -> 'a3 option) -> 'a1 option -> 'a2 option -> 'a3 option
 
 val pexpr_times_nformula :
-  'a1 -> 'a1 -> ('a1 -> 'a1 -> 'a1) -> ('a1 -> 'a1 -> 'a1) -> ('a1 -> 'a1 -> bool) -> 'a1 polC -> 'a1 nFormula -> 'a1 nFormula option
+  'a1 -> 'a1 -> ('a1 -> 'a1 -> 'a1) -> ('a1 -> 'a1 -> 'a1) -> ('a1 -> 'a1 -> bool) ->
+  'a1 polC -> 'a1 nFormula -> 'a1 nFormula option
 
 val nformula_times_nformula :
-  'a1 -> 'a1 -> ('a1 -> 'a1 -> 'a1) -> ('a1 -> 'a1 -> 'a1) -> ('a1 -> 'a1 -> bool) -> 'a1 nFormula -> 'a1 nFormula -> 'a1 nFormula option
+  'a1 -> 'a1 -> ('a1 -> 'a1 -> 'a1) -> ('a1 -> 'a1 -> 'a1) -> ('a1 -> 'a1 -> bool) ->
+  'a1 nFormula -> 'a1 nFormula -> 'a1 nFormula option
 
-val nformula_plus_nformula : 'a1 -> ('a1 -> 'a1 -> 'a1) -> ('a1 -> 'a1 -> bool) -> 'a1 nFormula -> 'a1 nFormula -> 'a1 nFormula option
+val nformula_plus_nformula :
+  'a1 -> ('a1 -> 'a1 -> 'a1) -> ('a1 -> 'a1 -> bool) -> 'a1 nFormula -> 'a1 nFormula
+  -> 'a1 nFormula option
 
 val eval_Psatz :
-  'a1 -> 'a1 -> ('a1 -> 'a1 -> 'a1) -> ('a1 -> 'a1 -> 'a1) -> ('a1 -> 'a1 -> bool) -> ('a1 -> 'a1 -> bool) -> 'a1 nFormula list -> 'a1 psatz -> 'a1
-  nFormula option
+  'a1 -> 'a1 -> ('a1 -> 'a1 -> 'a1) -> ('a1 -> 'a1 -> 'a1) -> ('a1 -> 'a1 -> bool) ->
+  ('a1 -> 'a1 -> bool) -> 'a1 nFormula list -> 'a1 psatz -> 'a1 nFormula option
 
-val check_inconsistent : 'a1 -> ('a1 -> 'a1 -> bool) -> ('a1 -> 'a1 -> bool) -> 'a1 nFormula -> bool
+val check_inconsistent :
+  'a1 -> ('a1 -> 'a1 -> bool) -> ('a1 -> 'a1 -> bool) -> 'a1 nFormula -> bool
 
 val check_normalised_formulas :
-  'a1 -> 'a1 -> ('a1 -> 'a1 -> 'a1) -> ('a1 -> 'a1 -> 'a1) -> ('a1 -> 'a1 -> bool) -> ('a1 -> 'a1 -> bool) -> 'a1 nFormula list -> 'a1 psatz -> bool
+  'a1 -> 'a1 -> ('a1 -> 'a1 -> 'a1) -> ('a1 -> 'a1 -> 'a1) -> ('a1 -> 'a1 -> bool) ->
+  ('a1 -> 'a1 -> bool) -> 'a1 nFormula list -> 'a1 psatz -> bool
 
 type op2 =
 | OpEq
@@ -300,27 +396,31 @@ type op2 =
 type 't formula = { flhs : 't pExpr; fop : op2; frhs : 't pExpr }
 
 val norm :
-  'a1 -> 'a1 -> ('a1 -> 'a1 -> 'a1) -> ('a1 -> 'a1 -> 'a1) -> ('a1 -> 'a1 -> 'a1) -> ('a1 -> 'a1) -> ('a1 -> 'a1 -> bool) -> 'a1 pExpr -> 'a1 pol
+  'a1 -> 'a1 -> ('a1 -> 'a1 -> 'a1) -> ('a1 -> 'a1 -> 'a1) -> ('a1 -> 'a1 -> 'a1) ->
+  ('a1 -> 'a1) -> ('a1 -> 'a1 -> bool) -> 'a1 pExpr -> 'a1 pol
 
-val psub0 : 'a1 -> ('a1 -> 'a1 -> 'a1) -> ('a1 -> 'a1 -> 'a1) -> ('a1 -> 'a1) -> ('a1 -> 'a1 -> bool) -> 'a1 pol -> 'a1 pol -> 'a1 pol
+val psub0 :
+  'a1 -> ('a1 -> 'a1 -> 'a1) -> ('a1 -> 'a1 -> 'a1) -> ('a1 -> 'a1) -> ('a1 -> 'a1 ->
+  bool) -> 'a1 pol -> 'a1 pol -> 'a1 pol
 
-val padd0 : 'a1 -> ('a1 -> 'a1 -> 'a1) -> ('a1 -> 'a1 -> bool) -> 'a1 pol -> 'a1 pol -> 'a1 pol
+val padd0 :
+  'a1 -> ('a1 -> 'a1 -> 'a1) -> ('a1 -> 'a1 -> bool) -> 'a1 pol -> 'a1 pol -> 'a1 pol
 
 val xnormalise :
-  'a1 -> 'a1 -> ('a1 -> 'a1 -> 'a1) -> ('a1 -> 'a1 -> 'a1) -> ('a1 -> 'a1 -> 'a1) -> ('a1 -> 'a1) -> ('a1 -> 'a1 -> bool) -> 'a1 formula -> 'a1
-  nFormula list
+  'a1 -> 'a1 -> ('a1 -> 'a1 -> 'a1) -> ('a1 -> 'a1 -> 'a1) -> ('a1 -> 'a1 -> 'a1) ->
+  ('a1 -> 'a1) -> ('a1 -> 'a1 -> bool) -> 'a1 formula -> 'a1 nFormula list
 
 val cnf_normalise :
-  'a1 -> 'a1 -> ('a1 -> 'a1 -> 'a1) -> ('a1 -> 'a1 -> 'a1) -> ('a1 -> 'a1 -> 'a1) -> ('a1 -> 'a1) -> ('a1 -> 'a1 -> bool) -> 'a1 formula -> 'a1
-  nFormula cnf
+  'a1 -> 'a1 -> ('a1 -> 'a1 -> 'a1) -> ('a1 -> 'a1 -> 'a1) -> ('a1 -> 'a1 -> 'a1) ->
+  ('a1 -> 'a1) -> ('a1 -> 'a1 -> bool) -> 'a1 formula -> 'a2 -> ('a1 nFormula, 'a2) cnf
 
 val xnegate :
-  'a1 -> 'a1 -> ('a1 -> 'a1 -> 'a1) -> ('a1 -> 'a1 -> 'a1) -> ('a1 -> 'a1 -> 'a1) -> ('a1 -> 'a1) -> ('a1 -> 'a1 -> bool) -> 'a1 formula -> 'a1
-  nFormula list
+  'a1 -> 'a1 -> ('a1 -> 'a1 -> 'a1) -> ('a1 -> 'a1 -> 'a1) -> ('a1 -> 'a1 -> 'a1) ->
+  ('a1 -> 'a1) -> ('a1 -> 'a1 -> bool) -> 'a1 formula -> 'a1 nFormula list
 
 val cnf_negate :
-  'a1 -> 'a1 -> ('a1 -> 'a1 -> 'a1) -> ('a1 -> 'a1 -> 'a1) -> ('a1 -> 'a1 -> 'a1) -> ('a1 -> 'a1) -> ('a1 -> 'a1 -> bool) -> 'a1 formula -> 'a1
-  nFormula cnf
+  'a1 -> 'a1 -> ('a1 -> 'a1 -> 'a1) -> ('a1 -> 'a1 -> 'a1) -> ('a1 -> 'a1 -> 'a1) ->
+  ('a1 -> 'a1) -> ('a1 -> 'a1 -> bool) -> 'a1 formula -> 'a2 -> ('a1 nFormula, 'a2) cnf
 
 val xdenorm : positive -> 'a1 pol -> 'a1 pExpr
 
@@ -330,7 +430,15 @@ val map_PExpr : ('a2 -> 'a1) -> 'a2 pExpr -> 'a1 pExpr
 
 val map_Formula : ('a2 -> 'a1) -> 'a2 formula -> 'a1 formula
 
-val simpl_cone : 'a1 -> 'a1 -> ('a1 -> 'a1 -> 'a1) -> ('a1 -> 'a1 -> bool) -> 'a1 psatz -> 'a1 psatz
+val simpl_cone :
+  'a1 -> 'a1 -> ('a1 -> 'a1 -> 'a1) -> ('a1 -> 'a1 -> bool) -> 'a1 psatz -> 'a1 psatz
+
+module PositiveSet :
+ sig
+  type tree =
+  | Leaf
+  | Node of tree * bool * tree
+ end
 
 type q = { qnum : z; qden : positive }
 
@@ -358,8 +466,8 @@ val qpower : q -> z -> q
 
 type 'a t =
 | Empty
-| Leaf of 'a
-| Node of 'a t * 'a * 'a t
+| Elt of 'a
+| Branch of 'a t * 'a * 'a t
 
 val find : 'a1 -> 'a1 t -> positive -> 'a1
 
@@ -379,15 +487,17 @@ val normZ : z pExpr -> z pol
 
 val xnormalise0 : z formula -> z nFormula list
 
-val normalise : z formula -> z nFormula cnf
+val normalise : z formula -> 'a1 -> (z nFormula, 'a1) cnf
 
 val xnegate0 : z formula -> z nFormula list
 
-val negate : z formula -> z nFormula cnf
+val negate : z formula -> 'a1 -> (z nFormula, 'a1) cnf
 
 val zunsat : z nFormula -> bool
 
 val zdeduce : z nFormula -> z nFormula -> z nFormula option
+
+val cnfZ : (z formula, 'a1, 'a2, 'a3) tFormula -> (z nFormula, 'a1) cnf * 'a1 list
 
 val ceiling : z -> z -> z
 
@@ -415,6 +525,51 @@ val eval_Psatz0 : z nFormula list -> zWitness -> z nFormula option
 
 val valid_cut_sign : op1 -> bool
 
+module Vars :
+ sig
+  type elt = positive
+
+  type tree = PositiveSet.tree =
+  | Leaf
+  | Node of tree * bool * tree
+
+  type t = tree
+
+  val empty : t
+
+  val add : elt -> t -> t
+
+  val singleton : elt -> t
+
+  val union : t -> t -> t
+
+  val rev_append : elt -> elt -> elt
+
+  val rev : elt -> elt
+
+  val xfold : (elt -> 'a1 -> 'a1) -> t -> 'a1 -> elt -> 'a1
+
+  val fold : (elt -> 'a1 -> 'a1) -> t -> 'a1 -> 'a1
+ end
+
+val vars_of_pexpr : z pExpr -> Vars.t
+
+val vars_of_formula : z formula -> Vars.t
+
+val vars_of_bformula : (z formula, 'a1, 'a2, 'a3) gFormula -> Vars.t
+
+val bound_var : positive -> z formula
+
+val mk_eq_pos : positive -> positive -> positive -> z formula
+
+val bound_vars :
+  (positive -> positive -> bool option -> 'a2) -> positive -> Vars.t -> (z formula,
+  'a1, 'a2, 'a3) gFormula
+
+val bound_problem_fr :
+  (positive -> positive -> bool option -> 'a2) -> positive -> (z formula, 'a1, 'a2,
+  'a3) gFormula -> (z formula, 'a1, 'a2, 'a3) gFormula
+
 val zChecker : z nFormula list -> zArithProof -> bool
 
 val zTautoChecker : z formula bFormula -> zArithProof list -> bool
@@ -423,15 +578,17 @@ type qWitness = q psatz
 
 val qWeakChecker : q nFormula list -> q psatz -> bool
 
-val qnormalise : q formula -> q nFormula cnf
+val qnormalise : q formula -> 'a1 -> (q nFormula, 'a1) cnf
 
-val qnegate : q formula -> q nFormula cnf
+val qnegate : q formula -> 'a1 -> (q nFormula, 'a1) cnf
 
 val qunsat : q nFormula -> bool
 
 val qdeduce : q nFormula -> q nFormula -> q nFormula option
 
 val normQ : q pExpr -> q pol
+
+val cnfQ : (q formula, 'a1, 'a2, 'a3) tFormula -> (q nFormula, 'a1) cnf * 'a1 list
 
 val qTautoChecker : q formula bFormula -> qWitness list -> bool
 
@@ -443,8 +600,11 @@ type rcst =
 | CPlus of rcst * rcst
 | CMinus of rcst * rcst
 | CMult of rcst * rcst
+| CPow of rcst * (z, nat) sum
 | CInv of rcst
 | COpp of rcst
+
+val z_of_exp : (z, nat) sum -> z
 
 val q_of_Rcst : rcst -> q
 
@@ -452,9 +612,9 @@ type rWitness = q psatz
 
 val rWeakChecker : q nFormula list -> q psatz -> bool
 
-val rnormalise : q formula -> q nFormula cnf
+val rnormalise : q formula -> 'a1 -> (q nFormula, 'a1) cnf
 
-val rnegate : q formula -> q nFormula cnf
+val rnegate : q formula -> 'a1 -> (q nFormula, 'a1) cnf
 
 val runsat : q nFormula -> bool
 
