plugins/micromega/RMicromega.v
@@ -17,10 +17,11 @@
 Require Import OrderedRing.
 Require Import RingMicromega.
 Require Import Refl.
-Require Import Raxioms RIneq Rpow_def DiscrR.
+Require Import Raxioms Rfunctions RIneq Rpow_def DiscrR.
 Require Import QArith.
 Require Import Qfield.
 Require Import Qreals.
+Require Import DeclConstant.
 
 Require Setoid.
 (*Declare ML Module "micromega_plugin".*)
@@ -57,8 +58,6 @@ Proof.
   now apply Rmult_lt_0_compat.
 Qed.
 
-Notation IQR := Q2R (only parsing).
-
 Lemma Rinv_1 : forall x, x * / 1 = x.
 Proof.
   intro.
@@ -66,13 +65,13 @@ Proof.
   apply Rmult_1_r.
 Qed.
 
-Lemma Qeq_true : forall x y, Qeq_bool x y = true -> IQR x = IQR y.
+Lemma Qeq_true : forall x y, Qeq_bool x y = true -> Q2R x = Q2R y.
 Proof.
   intros.
   now apply Qeq_eqR, Qeq_bool_eq.
 Qed.
 
-Lemma Qeq_false : forall x y, Qeq_bool x y = false -> IQR x <> IQR y.
+Lemma Qeq_false : forall x y, Qeq_bool x y = false -> Q2R x <> Q2R y.
 Proof.
   intros.
   apply Qeq_bool_neq in H.
@@ -80,24 +79,24 @@ Proof.
   now apply eqR_Qeq.
 Qed.
 
-Lemma Qle_true : forall x y : Q, Qle_bool x y = true -> IQR x <= IQR y.
+Lemma Qle_true : forall x y : Q, Qle_bool x y = true -> Q2R x <= Q2R y.
 Proof.
   intros.
   now apply Qle_Rle, Qle_bool_imp_le.
 Qed.
 
-Lemma IQR_0 : IQR 0 = 0.
+Lemma Q2R_0 : Q2R 0 = 0.
 Proof.
   apply Rmult_0_l.
 Qed.
 
-Lemma IQR_1 : IQR 1 = 1.
+Lemma Q2R_1 : Q2R 1 = 1.
 Proof.
   compute. apply Rinv_1.
 Qed.
 
-Lemma IQR_inv_ext : forall x, 
-  IQR (/ x) = (if Qeq_bool x 0 then 0 else / IQR x).
+Lemma Q2R_inv_ext : forall x,
+  Q2R (/ x) = (if Qeq_bool x 0 then 0 else / Q2R x).
 Proof.
   intros.
   case_eq (Qeq_bool x 0).
@@ -120,12 +119,12 @@ Lemma QSORaddon :
   R0 R1 Rplus Rmult Rminus Ropp  (@eq R)  Rle (* ring elements *)
   Q 0%Q 1%Q Qplus Qmult Qminus Qopp (* coefficients *)
   Qeq_bool Qle_bool
-  IQR nat to_nat pow.
+  Q2R nat to_nat pow.
 Proof.
   constructor.
   constructor ; intros ; try reflexivity.
-  apply IQR_0.
-  apply IQR_1.
+  apply Q2R_0.
+  apply Q2R_1.
   apply Q2R_plus.
   apply Q2R_minus.
   apply Q2R_mult.
@@ -136,20 +135,27 @@ Proof.
   apply Qle_true.
 Qed.
 
+(* Syntactic ring coefficients. *)
 
-(* Syntactic ring coefficients. 
-   For computing, we use Q. *)
 Inductive Rcst :=
-| C0
-| C1
-| CQ (r : Q)
-| CZ (r : Z)
-| CPlus (r1 r2 : Rcst)
-| CMinus (r1  r2 : Rcst)
-| CMult (r1 r2 : Rcst)
-| CInv  (r : Rcst)
-| COpp  (r : Rcst).
+  | C0
+  | C1
+  | CQ (r : Q)
+  | CZ (r : Z)
+  | CPlus (r1 r2 : Rcst)
+  | CMinus (r1  r2 : Rcst)
+  | CMult (r1 r2 : Rcst)
+  | CPow  (r1 : Rcst) (z:Z+nat)
+  | CInv  (r : Rcst)
+  | COpp  (r : Rcst).
 
+
+
+Definition z_of_exp (z : Z + nat) :=
+  match z with
+  | inl z => z
+  | inr n => Z.of_nat n
+  end.
 
 Fixpoint Q_of_Rcst (r : Rcst) : Q :=
   match r with
@@ -160,42 +166,198 @@ Fixpoint Q_of_Rcst (r : Rcst) : Q :=
     | CPlus r1 r2 => Qplus (Q_of_Rcst r1) (Q_of_Rcst r2)
     | CMinus r1 r2 => Qminus (Q_of_Rcst r1) (Q_of_Rcst r2)
     | CMult r1 r2  => Qmult (Q_of_Rcst r1) (Q_of_Rcst r2)
-    | CInv r        => Qinv (Q_of_Rcst r)
+    | CPow  r1 z   => Qpower (Q_of_Rcst r1) (z_of_exp z)
+    | CInv r       => Qinv (Q_of_Rcst r)
     | COpp r       => Qopp (Q_of_Rcst r)
   end.
 
+
+Definition is_neg (z: Z+nat) :=
+  match z with
+  | inl (Zneg _) => true
+  |  _           => false
+  end.
+
+Lemma is_neg_true : forall z, is_neg z = true -> (z_of_exp z < 0)%Z.
+Proof.
+  destruct z ; simpl ; try congruence.
+  destruct z ; try congruence.
+  intros.
+  reflexivity.
+Qed.
+
+Lemma is_neg_false : forall z, is_neg z = false -> (z_of_exp z >= 0)%Z.
+Proof.
+  destruct z ; simpl ; try congruence.
+  destruct z ; try congruence.
+  compute. congruence.
+  compute. congruence.
+  generalize (Zle_0_nat n). auto with zarith.
+Qed.
+
+Definition CInvR0 (r : Rcst) := Qeq_bool (Q_of_Rcst r) (0 # 1).
+
+Definition CPowR0 (z : Z) (r : Rcst) :=
+  Z.ltb z Z0 && Qeq_bool (Q_of_Rcst r) (0 # 1).
 
 Fixpoint R_of_Rcst (r : Rcst) : R :=
   match r with
     | C0 => R0
     | C1 => R1
     | CZ z => IZR z
-    | CQ q => IQR q
+    | CQ q => Q2R q
     | CPlus r1 r2  => (R_of_Rcst r1) + (R_of_Rcst r2)
     | CMinus r1 r2 => (R_of_Rcst r1) - (R_of_Rcst r2)
     | CMult r1 r2  => (R_of_Rcst r1) * (R_of_Rcst r2)
+    | CPow r1 z    =>
+      match z with
+      | inl z =>
+        if CPowR0 z r1
+        then R0
+        else  powerRZ (R_of_Rcst r1) z
+      | inr n => pow (R_of_Rcst r1) n
+      end
     | CInv r       => 
-      if Qeq_bool (Q_of_Rcst r) (0 # 1)
-        then R0 
-        else Rinv (R_of_Rcst r)
-      | COpp r       => - (R_of_Rcst r)
+      if CInvR0 r then R0
+      else Rinv (R_of_Rcst r)
+    | COpp r       => - (R_of_Rcst r)
   end.
 
-Lemma Q_of_RcstR : forall c, IQR (Q_of_Rcst c) = R_of_Rcst c.
+Add Morphism Q2R with signature Qeq ==> @eq R as Q2R_m.
+  exact Qeq_eqR.
+Qed.
+
+Lemma Q2R_pow_pos : forall q p,
+    Q2R (pow_pos Qmult q p) = pow_pos Rmult (Q2R q) p.
 Proof.
-    induction c ; simpl ; try (rewrite <- IHc1 ; rewrite <- IHc2).
-    apply IQR_0. 
-    apply IQR_1. 
+  induction p ; simpl;auto;
+    rewrite <- IHp;
+    repeat rewrite Q2R_mult;
     reflexivity.
-    unfold IQR. simpl. rewrite Rinv_1. reflexivity.
-    apply Q2R_plus.
-    apply Q2R_minus.
-    apply Q2R_mult.
-    rewrite <- IHc.
-    apply IQR_inv_ext.
-    rewrite <- IHc.
+Qed.
+
+Lemma Q2R_pow_N : forall q n,
+  Q2R (pow_N 1%Q Qmult q n) = pow_N 1 Rmult (Q2R q) n.
+Proof.
+  destruct n ; simpl.
+  - apply Q2R_1.
+  - apply Q2R_pow_pos.
+Qed.
+
+Lemma Qmult_integral : forall q r, q * r ==  0 -> q == 0 \/ r == 0.
+Proof.
+  intros.
+  destruct (Qeq_dec q 0)%Q.
+  - left ; apply q0.
+  - apply Qmult_integral_l in H ; tauto.
+Qed.
+
+Lemma Qpower_positive_eq_zero : forall q p,
+    Qpower_positive q p == 0 -> q == 0.
+Proof.
+  unfold Qpower_positive.
+  induction p ; simpl; intros;
+    repeat match goal with
+    | H : _ * _ == 0 |- _ =>
+      apply Qmult_integral in H; destruct H
+    end; tauto.
+Qed.
+
+Lemma Qpower_positive_zero : forall p,
+    Qpower_positive 0 p == 0%Q.
+Proof.
+  induction p ; simpl;
+    try rewrite IHp ; reflexivity.
+Qed.
+
+
+Lemma Q2RpowerRZ :
+  forall q z
+         (DEF : not (q == 0)%Q \/ (z >= Z0)%Z),
+    Q2R (q ^ z) = powerRZ (Q2R q) z.
+Proof.
+  intros.
+  destruct Qpower_theory.
+  destruct R_power_theory.
+  unfold Qpower, powerRZ.
+  destruct z.
+  - apply Q2R_1.
+  -
+    change (Qpower_positive q p)
+          with (Qpower q (Zpos p)).
+    rewrite <- N2Z.inj_pos.
+    rewrite <- positive_N_nat.
+    rewrite rpow_pow_N.
+    rewrite rpow_pow_N0.
+    apply Q2R_pow_N.
+  -
+    rewrite  Q2R_inv.
+    unfold Qpower_positive.
+    rewrite <- positive_N_nat.
+    rewrite rpow_pow_N0.
+    unfold pow_N.
+    rewrite Q2R_pow_pos.
+    auto.
+    intro.
+    apply Qpower_positive_eq_zero in H.
+    destruct DEF ; auto with arith.
+Qed.
+
+Lemma Qpower0 : forall z, (z <> 0)%Z -> (0 ^ z == 0)%Q.
+Proof.
+  unfold Qpower.
+  destruct z;intros.
+  - congruence.
+  - apply Qpower_positive_zero.
+  - rewrite Qpower_positive_zero.
+    reflexivity.
+Qed.
+
+
+Lemma Q_of_RcstR : forall c, Q2R (Q_of_Rcst c) = R_of_Rcst c.
+Proof.
+  induction c ; simpl ; try (rewrite <- IHc1 ; rewrite <- IHc2).
+  - apply Q2R_0.
+  - apply Q2R_1.
+  - reflexivity.
+  - unfold Q2R. simpl. rewrite Rinv_1. reflexivity.
+  - apply Q2R_plus.
+  - apply Q2R_minus.
+  - apply Q2R_mult.
+  - destruct z.
+    destruct (CPowR0 z c) eqn:C; unfold CPowR0 in C.
+    +
+      rewrite andb_true_iff in C.
+      destruct C as (C1 & C2).
+      rewrite Z.ltb_lt in C1.
+      apply Qeq_bool_eq in C2.
+      rewrite C2.
+      simpl.
+      rewrite Qpower0 by auto with zarith.
+      apply Q2R_0.
+    + rewrite Q2RpowerRZ.
+      rewrite IHc.
+      reflexivity.
+      rewrite andb_false_iff in C.
+      destruct C.
+      simpl. apply Z.ltb_ge in H.
+      auto with zarith.
+      left ; apply Qeq_bool_neq; auto.
+    + simpl.
+      rewrite <- IHc.
+      destruct Qpower_theory.
+      rewrite <- nat_N_Z.
+      rewrite rpow_pow_N.
+      destruct R_power_theory.
+      rewrite <- (Nnat.Nat2N.id n) at 2.
+      rewrite rpow_pow_N0.
+      apply Q2R_pow_N.
+  - rewrite <- IHc.
+    unfold CInvR0.
+    apply Q2R_inv_ext.
+  - rewrite <- IHc.
     apply Q2R_opp.
-  Qed.
+Qed.
 
 Require Import EnvRing.
 
@@ -227,7 +389,7 @@ Definition Reval_formula' :=
   eval_sformula  Rplus Rmult Rminus Ropp (@eq R) Rle Rlt N.to_nat pow R_of_Rcst.
 
 Definition QReval_formula := 
-  eval_formula  Rplus Rmult Rminus Ropp (@eq R) Rle Rlt IQR N.to_nat pow .
+  eval_formula  Rplus Rmult Rminus Ropp (@eq R) Rle Rlt Q2R N.to_nat pow .
 
 Lemma Reval_formula_compat : forall env f, Reval_formula env f <-> Reval_formula' env f.
 Proof.
@@ -242,12 +404,12 @@ Proof.
 Qed.
 
 Definition Qeval_nformula :=
-  eval_nformula 0 Rplus Rmult  (@eq R) Rle Rlt IQR.
+  eval_nformula 0 Rplus Rmult  (@eq R) Rle Rlt Q2R.
 
 
 Lemma Reval_nformula_dec : forall env d, (Qeval_nformula env d) \/ ~ (Qeval_nformula env d).
 Proof.
-  exact (fun env d =>eval_nformula_dec Rsor IQR env d).
+  exact (fun env d =>eval_nformula_dec Rsor Q2R env d).
 Qed.
 
 Definition RWitness := Psatz Q.
@@ -279,32 +441,41 @@ Definition rdeduce := nformula_plus_nformula 0%Q Qplus Qeq_bool.
 
 Definition RTautoChecker (f : BFormula (Formula Rcst)) (w: list RWitness)  : bool :=
   @tauto_checker (Formula Q) (NFormula Q)
-  runsat rdeduce
-  Rnormalise Rnegate
-  RWitness RWeakChecker (map_bformula (map_Formula Q_of_Rcst)  f) w.
+  unit runsat rdeduce
+  (Rnormalise unit) (Rnegate unit)
+  RWitness (fun cl => RWeakChecker (List.map fst cl)) (map_bformula (map_Formula Q_of_Rcst)  f) w.
 
-Lemma RTautoChecker_sound : forall f w, RTautoChecker f w = true -> forall env, eval_f  (Reval_formula env)  f.
+Lemma RTautoChecker_sound : forall f w, RTautoChecker f w = true -> forall env, eval_bf  (Reval_formula env)  f.
 Proof.
   intros f w.
   unfold RTautoChecker.
   intros TC env.
-  apply (tauto_checker_sound  QReval_formula Qeval_nformula) with (env := env) in TC.
-  rewrite eval_f_map in TC.
-  rewrite eval_f_morph with (ev':= Reval_formula env) in TC ; auto.
+  apply tauto_checker_sound with (eval:=QReval_formula) (eval':=    Qeval_nformula) (env := env) in TC.
+  - change (eval_f (fun x : Prop => x) (QReval_formula env))
+      with
+        (eval_bf  (QReval_formula env)) in TC.
+    rewrite eval_bf_map in TC.
+    unfold eval_bf in TC.
+    rewrite eval_f_morph with (ev':= Reval_formula env) in TC ; auto.
   intro.
   unfold QReval_formula.
   rewrite <- eval_formulaSC  with (phiS := R_of_Rcst).
   rewrite Reval_formula_compat.
   tauto.
   intro. rewrite Q_of_RcstR. reflexivity.
+  -
   apply Reval_nformula_dec.
-  destruct t.
+  - destruct t.
   apply (check_inconsistent_sound Rsor QSORaddon) ; auto.
-  unfold rdeduce. apply (nformula_plus_nformula_correct Rsor QSORaddon).
-  now apply (cnf_normalise_correct Rsor QSORaddon).  
-  intros. now apply (cnf_negate_correct Rsor QSORaddon).
-  intros t w0.
-  apply RWeakChecker_sound.
+  - unfold rdeduce. apply (nformula_plus_nformula_correct Rsor QSORaddon).
+  - now apply (cnf_normalise_correct Rsor QSORaddon).
+  - intros. now eapply (cnf_negate_correct Rsor QSORaddon); eauto.
+  - intros t w0.
+    unfold eval_tt.
+    intros.
+    rewrite make_impl_map with (eval := Qeval_nformula env0).
+    eapply RWeakChecker_sound; eauto.
+    tauto.
 Qed.
 
 
