plugins/micromega/Tauto.v
@@ -10,7 +10,7 @@
 (*                                                                      *)
 (* Micromega: A reflexive tactic using the Positivstellensatz           *)
 (*                                                                      *)
-(*  Frédéric Besson (Irisa/Inria) 2006-20011                            *)
+(*  Frédéric Besson (Irisa/Inria) 2006-20019                            *)
 (*                                                                      *)
 (************************************************************************)
 
@@ -21,176 +21,363 @@ Require Import Bool.
 Set Implicit Arguments.
 
 
-  #[universes(template)]
-  Inductive BFormula (A:Type) : Type :=
-  | TT   : BFormula A
-  | FF   : BFormula A
-  | X : Prop -> BFormula A
-  | A : A -> BFormula A
-  | Cj  : BFormula A -> BFormula A -> BFormula A
-  | D   : BFormula A-> BFormula A -> BFormula A
-  | N  : BFormula A -> BFormula A
-  | I : BFormula A-> BFormula A-> BFormula A.
+Section S.
+  Context {TA  : Type}. (* type of interpreted atoms *)
+  Context {TX  : Type}. (* type of uninterpreted terms (Prop) *)
+  Context {AA  : Type}. (* type of annotations for atoms *)
+  Context {AF  : Type}. (* type of formulae identifiers *)
 
-  Fixpoint eval_f (A:Type)  (ev:A -> Prop ) (f:BFormula A) {struct f}: Prop :=
-    match f with
-      | TT _ => True
-      | FF _ => False
-      | A a =>  ev a
-      | X _ p => p
-      | Cj e1 e2 => (eval_f  ev e1) /\ (eval_f ev e2)
-      | D e1 e2  => (eval_f  ev e1) \/ (eval_f  ev e2)
-      | N e     => ~ (eval_f  ev e)
-      | I f1 f2 => (eval_f  ev f1) -> (eval_f  ev f2)
+  #[universes(template)]
+   Inductive GFormula  : Type :=
+  | TT   : GFormula
+  | FF   : GFormula
+  | X    : TX -> GFormula
+  | A    : TA -> AA -> GFormula
+  | Cj   : GFormula  -> GFormula  -> GFormula
+  | D    : GFormula  -> GFormula  -> GFormula
+  | N    : GFormula  -> GFormula
+  | I    : GFormula  -> option AF -> GFormula  -> GFormula.
+
+  Section MAPX.
+    Variable F : TX -> TX.
+
+    Fixpoint mapX (f : GFormula) : GFormula :=
+      match f with
+      | TT => TT
+      | FF => FF
+      | X x => X (F x)
+      | A a an => A a an
+      | Cj f1 f2 => Cj (mapX f1) (mapX f2)
+      | D f1 f2  => D (mapX f1) (mapX f2)
+      | N f      => N (mapX f)
+      | I f1 o f2 => I (mapX f1) o (mapX f2)
+      end.
+
+  End MAPX.
+
+  Section FOLDANNOT.
+    Variable ACC : Type.
+    Variable F : ACC -> AA -> ACC.
+
+    Fixpoint foldA (f : GFormula) (acc : ACC) : ACC :=
+      match f with
+      | TT => acc
+      | FF => acc
+      | X x => acc
+      | A a an => F acc an
+      | Cj f1 f2
+      | D f1 f2
+      | I f1 _ f2 => foldA f1 (foldA f2 acc)
+      | N f      => foldA f acc
+      end.
+
+  End FOLDANNOT.
+
+
+  Definition cons_id (id : option AF) (l : list AF) :=
+    match id with
+    | None => l
+    | Some id => id :: l
     end.
 
-  Lemma eval_f_morph : forall  A (ev ev' : A -> Prop) (f : BFormula A),
-    (forall a, ev a <-> ev' a) -> (eval_f ev f <-> eval_f ev' f).
+  Fixpoint ids_of_formula f :=
+    match f with
+    | I f id f' => cons_id id (ids_of_formula f')
+    |  _           => nil
+    end.
+
+  Fixpoint collect_annot (f : GFormula) : list AA :=
+    match f with
+    | TT | FF | X _ => nil
+    | A _ a => a ::nil
+    | Cj f1 f2
+    | D  f1 f2
+    | I f1 _ f2  => collect_annot f1 ++ collect_annot f2
+    | N  f       => collect_annot f
+    end.
+
+  Variable ex : TX -> Prop. (* [ex] will be the identity *)
+
+  Section EVAL.
+
+  Variable ea : TA -> Prop.
+
+  Fixpoint eval_f (f:GFormula) {struct f}: Prop :=
+  match f with
+  | TT  => True
+  | FF  => False
+  | A a _ =>  ea a
+  | X  p => ex p
+  | Cj e1 e2 => (eval_f e1) /\ (eval_f e2)
+  | D e1 e2  => (eval_f e1) \/ (eval_f e2)
+  | N e     => ~ (eval_f e)
+  | I f1 _ f2 => (eval_f f1) -> (eval_f f2)
+  end.
+
+
+  End EVAL.
+
+
+
+
+
+  Lemma eval_f_morph :
+    forall  (ev ev' : TA -> Prop) (f : GFormula),
+      (forall a, ev a <-> ev' a) -> (eval_f ev f <-> eval_f ev' f).
   Proof.
     induction f ; simpl ; try tauto.
     intros.
-    assert (H' := H a).
-    auto.
+    apply H.
   Qed.
 
 
-
-  Fixpoint map_bformula (T U : Type) (fct : T -> U) (f : BFormula T) : BFormula U :=
-    match f with
-      | TT _ => TT _
-      | FF _ => FF _
-      | X _ p => X _ p
-      | A a => A (fct a)
-      | Cj f1 f2 => Cj (map_bformula fct f1) (map_bformula fct f2)
-      | D f1 f2 => D (map_bformula fct f1) (map_bformula fct f2)
-      | N f     => N (map_bformula fct f)
-      | I f1 f2 => I (map_bformula fct f1) (map_bformula fct f2)
-    end.
-
-  Lemma eval_f_map : forall T U (fct: T-> U) env f ,
-    eval_f env  (map_bformula fct f)  = eval_f (fun x => env (fct x)) f.
-  Proof.
-    induction f ; simpl ; try (rewrite IHf1 ; rewrite IHf2) ; auto.
-    rewrite <- IHf.  auto.    
-  Qed.
+End S.
 
 
 
-  Lemma map_simpl : forall A B f l, @map A B f l = match l with
+(** Typical boolean formulae *)
+Definition BFormula (A : Type) := @GFormula A Prop unit unit.
+
+Section MAPATOMS.
+  Context {TA TA':Type}.
+  Context {TX  : Type}.
+  Context {AA  : Type}.
+  Context {AF  : Type}.
+
+
+Fixpoint map_bformula (fct : TA -> TA') (f : @GFormula TA TX AA AF ) : @GFormula TA' TX AA AF :=
+  match f with
+  | TT  => TT
+  | FF  => FF
+  | X p => X  p
+  | A a t => A (fct a) t
+  | Cj f1 f2 => Cj (map_bformula fct f1) (map_bformula fct f2)
+  | D f1 f2 => D (map_bformula fct f1) (map_bformula fct f2)
+  | N f     => N (map_bformula fct f)
+  | I f1 a f2 => I (map_bformula fct f1) a (map_bformula fct f2)
+  end.
+
+End MAPATOMS.
+
+Lemma map_simpl : forall A B f l, @map A B f l = match l with
                                                  | nil => nil
                                                  | a :: l=> (f a) :: (@map A B f l)
-                                               end.
-  Proof.
-    destruct l ; reflexivity.
-  Qed.
+                                                 end.
+Proof.
+  destruct l ; reflexivity.
+Qed.
 
 
+Section S.
+  (** A cnf tracking annotations of atoms. *)
+
+  (** Type parameters *)
+  Variable Env   : Type.
+  Variable Term  : Type.
+  Variable Term' : Type.
+  Variable Annot : Type.
+
+  Variable unsat : Term'  -> bool. (* see [unsat_prop] *)
+  Variable deduce : Term' -> Term' -> option Term'. (* see [deduce_prop] *)
+
+  Definition clause := list  (Term' * Annot).
+  Definition cnf := list clause.
+
+  Variable normalise : Term -> Annot -> cnf.
+  Variable negate : Term -> Annot -> cnf.
 
 
-  Section S.
+  Definition cnf_tt : cnf := @nil clause.
+  Definition cnf_ff : cnf :=  cons (@nil (Term' * Annot)) nil.
 
-    Variable Env   : Type.
-    Variable Term  : Type.
-    Variable eval  : Env -> Term -> Prop.
-    Variable Term' : Type.
-    Variable eval'  : Env -> Term' -> Prop.
+  (** Our cnf is optimised and detects contradictions on the fly. *)
 
-
-
-    Variable no_middle_eval' : forall env d, (eval' env d) \/ ~ (eval' env d).
-
-    Variable unsat : Term'  -> bool.
-
-    Variable unsat_prop : forall t, unsat t  = true ->  
-      forall env, eval' env t -> False. 
-
-    Variable deduce : Term' -> Term' -> option Term'.
-
-    Variable deduce_prop : forall env t t' u,
-      eval' env t -> eval' env t' -> deduce t t' = Some u -> eval' env u.
-
-    Definition clause := list  Term'.
-    Definition cnf := list clause.
-
-    Variable normalise : Term -> cnf.
-    Variable negate : Term -> cnf.
-
-
-    Definition tt : cnf := @nil clause.
-    Definition ff : cnf :=  cons (@nil Term') nil.
-
-
-    Fixpoint add_term (t: Term') (cl : clause) : option clause :=
+  Fixpoint add_term (t: Term' * Annot) (cl : clause) : option clause :=
       match cl with
-        | nil => 
-          match deduce t t with
-            | None =>  Some (t ::nil)
-            | Some u => if unsat u then None else Some (t::nil)
+      | nil =>
+        match deduce (fst t) (fst t) with
+        | None =>  Some (t ::nil)
+        | Some u => if unsat u then None else Some (t::nil)
+        end
+      | t'::cl =>
+        match deduce (fst t) (fst t') with
+        | None =>
+          match add_term t cl with
+          | None => None
+          | Some cl' => Some (t' :: cl')
           end
-        | t'::cl => 
-          match deduce t t' with
-            | None => 
-              match add_term t cl with
-                | None => None
-                | Some cl' => Some (t' :: cl')
-              end
-            | Some u => 
-              if unsat u then None else 
-                match add_term t cl with
-                  | None => None
-                  | Some cl' => Some (t' :: cl')
-                end
-          end
+        | Some u =>
+          if unsat u then None else
+            match add_term t cl with
+            | None => None
+            | Some cl' => Some (t' :: cl')
+            end
+        end
       end.
 
     Fixpoint or_clause (cl1 cl2 : clause) : option clause :=
       match cl1 with
-        | nil => Some cl2
-        | t::cl => match add_term t cl2 with
-                     | None => None
-                     | Some cl' => or_clause cl cl'
-                   end
+      | nil => Some cl2
+      | t::cl => match add_term t cl2 with
+               | None => None
+               | Some cl' => or_clause cl cl'
+                 end
       end.
 
-(*    Definition or_clause_cnf (t:clause) (f:cnf) : cnf :=
-      List.map (fun x => (t++x)) f. *)
+    (*    Definition or_clause_cnf (t:clause) (f:cnf) : cnf :=
+          List.map (fun x => (t++x)) f. *)
 
     Definition or_clause_cnf (t:clause) (f:cnf) : cnf :=
-      List.fold_right (fun e acc => 
-        match or_clause t e with
-          | None => acc
-          | Some cl => cl :: acc
-        end) nil f.
+      List.fold_right (fun e acc =>
+                         match or_clause t e with
+                         | None => acc
+                         | Some cl => cl :: acc
+                         end) nil f.
 
 
     Fixpoint or_cnf (f : cnf) (f' : cnf) {struct f}: cnf :=
       match f with
-        | nil => tt
-        | e :: rst => (or_cnf rst f') ++ (or_clause_cnf e f')
+      | nil => cnf_tt
+      | e :: rst => (or_cnf rst f') ++ (or_clause_cnf e f')
       end.
 
 
     Definition and_cnf (f1 : cnf) (f2 : cnf) : cnf :=
       f1 ++ f2.
 
-    Fixpoint xcnf (pol : bool) (f : BFormula Term)  {struct f}: cnf :=
+    (** TX is Prop in Coq and EConstr.constr in Ocaml.
+      AF i s unit in Coq and Names.Id.t in Ocaml
+     *)
+    Definition TFormula (TX: Type) (AF: Type) := @GFormula Term TX Annot AF.
+
+    Fixpoint xcnf {TX AF: Type} (pol : bool) (f : TFormula TX AF)  {struct f}: cnf :=
       match f with
-        | TT _ => if pol then tt else ff
-        | FF _ => if pol then ff else tt
-        | X _ p => if pol then ff else ff (* This is not complete - cannot negate any proposition *)
-        | A x => if pol then normalise x else negate x
-        | N e  => xcnf (negb pol) e
-        | Cj e1 e2 =>
-          (if pol then and_cnf else or_cnf) (xcnf pol e1) (xcnf pol e2)
-        | D e1 e2  => (if pol then or_cnf else and_cnf) (xcnf pol e1) (xcnf pol e2)
-        | I e1 e2 => (if pol then or_cnf else and_cnf) (xcnf (negb pol) e1) (xcnf pol e2)
+      | TT  => if pol then cnf_tt else cnf_ff
+      | FF  => if pol then cnf_ff else cnf_tt
+      | X  p => if pol then cnf_ff else cnf_ff (* This is not complete - cannot negate any proposition *)
+      | A x t => if pol then normalise x  t else negate x  t
+      | N e  => xcnf (negb pol) e
+      | Cj e1 e2 =>
+        (if pol then and_cnf else or_cnf) (xcnf pol e1) (xcnf pol e2)
+      | D e1 e2  => (if pol then or_cnf else and_cnf) (xcnf pol e1) (xcnf pol e2)
+      | I e1 _ e2 => (if pol then or_cnf else and_cnf) (xcnf (negb pol) e1) (xcnf pol e2)
       end.
 
-    Definition eval_clause (env : Env) (cl : clause) := ~ make_conj  (eval' env) cl.
+    Section CNFAnnot.
+
+      (** Records annotations used to optimise the cnf.
+          Those need to be kept when pruning the formula.
+          For efficiency, this is a separate function.
+       *)
+
+
+
+      Fixpoint radd_term (t : Term' * Annot) (cl : clause) : clause + list Annot :=
+        match cl with
+        | nil => (* if t is unsat, the clause is empty BUT t is needed. *)
+          match deduce (fst t) (fst t) with
+          | Some u => if unsat u then inr ((snd t)::nil) else inl (t::nil)
+          | None   => inl (t::nil)
+          end
+        | t'::cl => (* if t /\ t' is unsat, the clause is empty BUT t & t' are needed *)
+          match deduce (fst t) (fst t') with
+          | Some u => if unsat u then inr ((snd t)::(snd t')::nil)
+                      else match radd_term t cl with
+                           | inl cl' => inl (t'::cl')
+                           | inr l   => inr l
+                           end
+          | None  => match radd_term t cl  with
+                     | inl cl' => inl (t'::cl')
+                     | inr l   => inr l
+                     end
+          end
+        end.
+
+      Fixpoint ror_clause cl1 cl2 :=
+        match cl1 with
+        | nil => inl cl2
+        | t::cl => match radd_term t cl2 with
+                   | inl cl' => ror_clause cl cl'
+                   | inr l   => inr l
+                   end
+        end.
+
+      Definition ror_clause_cnf t f :=
+        List.fold_right (fun e '(acc,tg) =>
+                           match ror_clause t e with
+                           | inl cl => (cl :: acc,tg)
+                           | inr l => (acc,tg++l)
+                           end) (nil,nil) f .
+
+
+      Fixpoint ror_cnf f f' :=
+        match f with
+        | nil => (cnf_tt,nil)
+        | e :: rst =>
+          let (rst_f',t) := ror_cnf rst f' in
+          let (e_f', t') := ror_clause_cnf e f' in
+          (rst_f' ++ e_f', t ++ t')
+        end.
+
+      Fixpoint rxcnf {TX AF: Type}(polarity : bool) (f : TFormula TX AF) :=
+        match f with
+        | TT => if polarity then (cnf_tt,nil) else (cnf_ff,nil)
+        | FF  => if polarity then (cnf_ff,nil) else (cnf_tt,nil)
+        | X p => if polarity then (cnf_ff,nil) else (cnf_ff,nil)
+        | A x t  => ((if polarity then normalise x t else negate x t),nil)
+        | N e  => rxcnf (negb polarity) e
+        | Cj e1 e2 =>
+          let (e1,t1) := rxcnf polarity e1 in
+          let (e2,t2) := rxcnf polarity e2 in
+          if polarity
+          then  (e1 ++ e2, t1 ++ t2)
+       else let (f',t') := ror_cnf e1 e2 in
+            (f', t1 ++ t2 ++ t')
+        | D e1 e2  =>
+          let (e1,t1) := rxcnf polarity e1 in
+          let (e2,t2) := rxcnf polarity e2 in
+          if polarity
+       then let (f',t') := ror_cnf e1 e2 in
+            (f', t1 ++ t2 ++ t')
+          else (e1 ++ e2, t1 ++ t2)
+        | I e1 _ e2 =>
+          let (e1 , t1) := (rxcnf (negb polarity) e1) in
+          let (e2 , t2) := (rxcnf polarity e2) in
+          if polarity
+          then let (f',t') := ror_cnf e1 e2 in
+               (f', t1 ++ t2 ++ t')
+          else (and_cnf e1 e2, t1 ++ t2)
+        end.
+
+      End CNFAnnot.
+
+
+
+    Variable eval  : Env -> Term -> Prop.
+
+    Variable eval'  : Env -> Term' -> Prop.
+
+    Variable no_middle_eval' : forall env d, (eval' env d) \/ ~ (eval' env d).
+
+
+    Variable unsat_prop : forall t, unsat t  = true ->
+                                    forall env, eval' env t -> False.
+
+
+
+    Variable deduce_prop : forall env t t' u,
+        eval' env t -> eval' env t' -> deduce t t' = Some u -> eval' env u.
+
+
+
+    Definition eval_tt (env : Env) (tt : Term' * Annot) := eval' env (fst tt).
+
+
+    Definition eval_clause (env : Env) (cl : clause) := ~ make_conj  (eval_tt env) cl.
 
     Definition eval_cnf (env : Env) (f:cnf) := make_conj  (eval_clause  env) f.
 
-    
+
     Lemma eval_cnf_app : forall env x y, eval_cnf env (x++y) -> eval_cnf env x /\ eval_cnf env y.
     Proof.
       unfold eval_cnf.
@@ -201,97 +388,107 @@ Set Implicit Arguments.
 
     Definition eval_opt_clause (env : Env) (cl: option clause) :=
       match cl with
-        | None => True
-        | Some cl => eval_clause env cl
+      | None => True
+      | Some cl => eval_clause env cl
       end.
 
 
-    Lemma add_term_correct : forall env t cl , eval_opt_clause env (add_term t cl) -> eval_clause env (t::cl).
-    Proof.
-      induction cl.
-      (* BC *)
-      simpl.
-      case_eq (deduce t t) ; auto.
-      intros *.
-      case_eq (unsat t0) ; auto.
-      unfold eval_clause.
-      rewrite make_conj_cons. 
-      intros. intro.
-      apply unsat_prop with (1:= H) (env := env).
-      apply deduce_prop with (3:= H0) ; tauto.
-      (* IC *)
-      simpl.
-      case_eq (deduce t a).
-      intro u.
-      case_eq (unsat u).
-      simpl. intros.
-      unfold eval_clause.
-      intro.
-      apply unsat_prop  with (1:= H) (env:= env).
-      repeat rewrite make_conj_cons in H2.
-      apply deduce_prop with (3:= H0); tauto.
-      intro.
-      case_eq (add_term t cl) ; intros.
-      simpl in H2.
-      rewrite H0 in IHcl.
-      simpl in IHcl.
-      unfold eval_clause in *.
-      intros.
-      repeat rewrite make_conj_cons in *.
-      tauto.
-      rewrite H0 in IHcl ; simpl in *.
-      unfold eval_clause in *.
-      intros.
-      repeat rewrite make_conj_cons in *.
-      tauto.
-      case_eq (add_term t cl) ; intros.
-      simpl in H1.
-      unfold eval_clause in *.
-      repeat rewrite make_conj_cons in *.
-      rewrite H in IHcl.
-      simpl in IHcl.
-      tauto.
-      simpl in *.
-      rewrite H in IHcl.
-      simpl in IHcl.
-      unfold eval_clause in *.
-      repeat rewrite make_conj_cons in *.    
-      tauto.
-    Qed.
+  Lemma add_term_correct : forall env t cl , eval_opt_clause env (add_term t cl) -> eval_clause env (t::cl).
+  Proof.
+    induction cl.
+    - (* BC *)
+    simpl.
+    case_eq (deduce (fst t) (fst t)) ; auto.
+    intros *.
+    case_eq (unsat t0) ; auto.
+    unfold eval_clause.
+    rewrite make_conj_cons.
+    intros. intro.
+    apply unsat_prop with (1:= H) (env := env).
+    apply deduce_prop with (3:= H0) ; tauto.
+    - (* IC *)
+    simpl.
+    case_eq (deduce (fst t) (fst a)).
+    intro u.
+    case_eq (unsat u).
+    simpl. intros.
+    unfold eval_clause.
+    intro.
+    apply unsat_prop  with (1:= H) (env:= env).
+    repeat rewrite make_conj_cons in H2.
+    apply deduce_prop with (3:= H0); tauto.
+    intro.
+    case_eq (add_term t cl) ; intros.
+    simpl in H2.
+    rewrite H0 in IHcl.
+    simpl in IHcl.
+    unfold eval_clause in *.
+    intros.
+    repeat rewrite make_conj_cons in *.
+    tauto.
+    rewrite H0 in IHcl ; simpl in *.
+    unfold eval_clause in *.
+    intros.
+    repeat rewrite make_conj_cons in *.
+    tauto.
+    case_eq (add_term t cl) ; intros.
+    simpl in H1.
+    unfold eval_clause in *.
+    repeat rewrite make_conj_cons in *.
+    rewrite H in IHcl.
+    simpl in IHcl.
+    tauto.
+    simpl in *.
+    rewrite H in IHcl.
+    simpl in IHcl.
+    unfold eval_clause in *.
+    repeat rewrite make_conj_cons in *.
+    tauto.
+  Qed.
 
+
+  Lemma no_middle_eval_tt : forall env a,
+      eval_tt env a \/ ~ eval_tt env a.
+  Proof.
+    unfold eval_tt.
+    auto.
+  Qed.
+
+  Hint Resolve no_middle_eval_tt : tauto.
 
   Lemma or_clause_correct : forall cl cl' env,  eval_opt_clause env (or_clause cl cl') -> eval_clause env cl \/ eval_clause env cl'.
   Proof.
     induction cl.
-    simpl. tauto.
-    intros *.
-    simpl.
-    assert (HH := add_term_correct env a cl').
-    case_eq (add_term a cl').
-    simpl in *.
-    intros.
-    apply IHcl in H0.
-    rewrite H in HH.
-    simpl in HH.
-    unfold eval_clause in *.
-    destruct H0.
-    repeat rewrite make_conj_cons in *.
-    tauto.
-    apply HH in H0.
-    apply not_make_conj_cons in H0 ; auto.
-    repeat rewrite make_conj_cons in *.
-    tauto.
-    simpl.
-    intros.
-    rewrite H in HH.
-    simpl in HH.
-    unfold eval_clause in *.
-    assert (HH' := HH Coq.Init.Logic.I).
-    apply not_make_conj_cons in HH'; auto.
-    repeat rewrite make_conj_cons in *.
-    tauto.
+    - simpl. tauto.
+    - intros *.
+      simpl.
+      assert (HH := add_term_correct env a cl').
+      case_eq (add_term a cl').
+      +
+      intros.
+      apply IHcl in H0.
+      rewrite H in HH.
+      simpl in HH.
+      unfold eval_clause in *.
+      destruct H0.
+      *
+      repeat rewrite make_conj_cons in *.
+      tauto.
+      * apply HH in H0.
+        apply not_make_conj_cons in H0 ; auto with tauto.
+        repeat rewrite make_conj_cons in *.
+        tauto.
+      +
+      intros.
+      rewrite H in HH.
+      simpl in HH.
+      unfold eval_clause in *.
+      assert (HH' := HH Coq.Init.Logic.I).
+      apply not_make_conj_cons in HH'; auto with tauto.
+      repeat rewrite make_conj_cons in *.
+      tauto.
   Qed.
-    
+
 
   Lemma or_clause_cnf_correct : forall env t f, eval_cnf env (or_clause_cnf t f) -> (eval_clause env t) \/ (eval_cnf env f).
   Proof.
@@ -299,39 +496,38 @@ Set Implicit Arguments.
     unfold or_clause_cnf.
     intros until t.
     set (F := (fun (e : clause) (acc : list clause) =>
-         match or_clause t e with
-         | Some cl => cl :: acc
-         | None => acc
-         end)).
-    induction f.
-    auto.
-    (**)
+                 match or_clause t e with
+                 | Some cl => cl :: acc
+                 | None => acc
+                 end)).
+    induction f;auto.
     simpl.
     intros.
     destruct f.
-    simpl in H.
-    simpl in IHf. 
-    unfold F in H.
-    revert H.
-    intros.
-    apply or_clause_correct.
-    destruct (or_clause t a) ; simpl in * ; auto.
-    unfold F in H at 1.
-    revert H.
-    assert (HH := or_clause_correct t a env).
-    destruct (or_clause t a); simpl in HH ;
-    rewrite make_conj_cons in * ; intuition.
-    rewrite make_conj_cons in *.
-    tauto.
+    -  simpl in H.
+       simpl in IHf.
+       unfold F in H.
+       revert H.
+       intros.
+       apply or_clause_correct.
+       destruct (or_clause t a) ; simpl in * ; auto.
+    -
+      unfold F in H at 1.
+      revert H.
+      assert (HH := or_clause_correct t a env).
+      destruct (or_clause t a); simpl in HH ;
+        rewrite make_conj_cons in * ; intuition.
+      rewrite make_conj_cons in *.
+      tauto.
   Qed.
 
 
- Lemma eval_cnf_cons : forall env a f,  (~ make_conj  (eval' env) a) -> eval_cnf env f -> eval_cnf env (a::f).
- Proof.
-   intros.
-   unfold eval_cnf in *.
-   rewrite make_conj_cons ; eauto.
- Qed.
+  Lemma eval_cnf_cons : forall env a f,  (~ make_conj  (eval_tt env) a) -> eval_cnf env f -> eval_cnf env (a::f).
+  Proof.
+    intros.
+    unfold eval_cnf in *.
+    rewrite make_conj_cons ; eauto.
+  Qed.
 
   Lemma or_cnf_correct : forall env f f', eval_cnf env (or_cnf f f') -> (eval_cnf env  f) \/ (eval_cnf  env f').
   Proof.
@@ -352,12 +548,11 @@ Set Implicit Arguments.
     right ; auto.
   Qed.
 
-  Variable normalise_correct : forall env t, eval_cnf  env (normalise t) -> eval env t.
+  Variable normalise_correct : forall env t tg, eval_cnf  env (normalise t tg) -> eval env t.
 
-  Variable negate_correct : forall env t, eval_cnf env (negate t) -> ~ eval env t.
+  Variable negate_correct : forall env t tg, eval_cnf env (negate t tg) -> ~ eval env t.
 
-
-  Lemma xcnf_correct : forall f pol env, eval_cnf env (xcnf pol f) -> eval_f (eval env) (if pol then f else N f).
+  Lemma xcnf_correct : forall (f : @GFormula Term Prop Annot unit)  pol env, eval_cnf env (xcnf pol f) -> eval_f (fun x => x) (eval env) (if pol then f else N f).
   Proof.
     induction f.
     (* TT *)
@@ -385,10 +580,10 @@ Set Implicit Arguments.
     simpl.
     destruct pol ; simpl.
     intros.
-    apply normalise_correct  ; auto.
+    eapply normalise_correct  ; eauto.
     (* A 2 *)
     intros.
-    apply  negate_correct ; auto.
+    eapply  negate_correct ; eauto.
     auto.
     (* Cj *)
     destruct pol ; simpl.
@@ -462,21 +657,21 @@ Set Implicit Arguments.
 
 
   Variable Witness : Type.
-  Variable checker : list Term' -> Witness -> bool.
+  Variable checker : list (Term'*Annot) -> Witness -> bool.
 
-  Variable checker_sound : forall t  w, checker t w = true -> forall env, make_impl (eval' env)  t False.
+  Variable checker_sound : forall t  w, checker t w = true -> forall env, make_impl (eval_tt env)  t False.
 
   Fixpoint cnf_checker (f : cnf) (l : list Witness)  {struct f}: bool :=
     match f with
-      | nil => true
-      | e::f => match l with
-                  | nil => false
-                  | c::l => match checker e c with
-                              | true => cnf_checker f l
-                              |   _  => false
-                            end
-                end
-      end.
+    | nil => true
+    | e::f => match l with
+              | nil => false
+              | c::l => match checker e c with
+                        | true => cnf_checker f l
+                        |   _  => false
+                        end
+              end
+    end.
 
   Lemma cnf_checker_sound : forall t  w, cnf_checker t w = true -> forall env, eval_cnf  env  t.
   Proof.
@@ -501,21 +696,31 @@ Set Implicit Arguments.
   Qed.
 
 
-  Definition tauto_checker (f:BFormula Term) (w:list Witness) : bool :=
+  Definition tauto_checker (f:@GFormula Term Prop Annot unit) (w:list Witness) : bool :=
     cnf_checker (xcnf true f) w.
 
-  Lemma tauto_checker_sound : forall t  w, tauto_checker t w = true -> forall env, eval_f  (eval env)  t.
+  Lemma tauto_checker_sound : forall t  w, tauto_checker t w = true -> forall env, eval_f (fun x => x) (eval env)  t.
   Proof.
     unfold tauto_checker.
     intros.
-    change (eval_f (eval env) t) with (eval_f (eval env) (if true then t else TT Term)).
+    change (eval_f (fun x => x) (eval env) t) with (eval_f (fun x => x) (eval env) (if true then t else TT)).
     apply (xcnf_correct t true).
     eapply cnf_checker_sound ; eauto.
   Qed.
 
+  Definition eval_bf {A : Type} (ea : A -> Prop) (f: BFormula A) := eval_f (fun x => x) ea f.
+
+
+  Lemma eval_bf_map : forall T U (fct: T-> U) env f ,
+    eval_bf env  (map_bformula fct f)  = eval_bf (fun x => env (fct x)) f.
+Proof.
+  induction f ; simpl ; try (rewrite IHf1 ; rewrite IHf2) ; auto.
+  rewrite <- IHf.  auto.
+Qed.
 
 
 End S.
+
 
 (* Local Variables: *)
 (* coding: utf-8 *)
