plugins/micromega/Lra.v
@@ -24,7 +24,7 @@ Declare ML Module "micromega_plugin".
 
 Ltac rchange := 
   intros __wit __varmap __ff ;
-  change (Tauto.eval_f (Reval_formula (@find R 0%R __varmap)) __ff) ;
+  change (Tauto.eval_bf (Reval_formula (@find R 0%R __varmap)) __ff) ;
   apply (RTautoChecker_sound __ff __wit).
 
 Ltac rchecker_no_abstract := rchange ; vm_compute ; reflexivity.
