test-suite/output/MExtraction.v
@@ -7,6 +7,8 @@ Require Import QMicromega.
 Require Import RMicromega.
 
 Recursive Extraction
-   List.map simpl_cone (*map_cone  indexes*)
-   denorm Qpower vm_add
+           Tauto.mapX Tauto.foldA Tauto.collect_annot Tauto.ids_of_formula Tauto.map_bformula
+           ZMicromega.cnfZ ZMicromega.bound_problem_fr QMicromega.cnfQ
+           List.map simpl_cone (*map_cone  indexes*)
+           denorm Qpower vm_add
    normZ normQ normQ n_of_Z N.of_nat ZTautoChecker ZWeakChecker QTautoChecker RTautoChecker find.
